src/Narcissus/BinLib/AlignedEncodeMonad.v
@@ -7,6 +7,7 @@ Require Import
         Coq.Logic.Eqdep_dec
         Fiat.Narcissus.Common.Specs
         Fiat.Narcissus.Common.ComposeOpt
+        Fiat.Narcissus.BaseFormats
         Fiat.Narcissus.BinLib.Core
         Fiat.Narcissus.BinLib.AlignedByteString.
 
@@ -113,20 +114,6 @@ Section AlignedEncodeM.
     | _, _ => @Vector.nil _
     end.
 
-  Definition SetCurrentByte (* Sets a single byte at the current index and increments the current index. *)
-             {n : nat}
-             (a : char)
-    : AlignedEncodeM n :=
-    fun v idx s ce => if (idx <? n) then Some (set_nth' v idx a, Datatypes.S idx, addE ce 8) else None.
-
-  Definition SetByteAt (* Sets the bytes at the specified index and sets the current index
-                          to the following position. *)
-             {n : nat}
-             (a : word 8)
-             (idx' : nat)
-    : AlignedEncodeM n :=
-    fun v idx s ce => if (NPeano.ltb idx' n) then Some (set_nth' v idx' a, Datatypes.S idx', addE ce 8) else None.
-
   (* Equivalence Criteria:
      A bit-aligned encoder and byte-aligned encoder are equivalent when
      - the byte aligned encoder fails when the bit aligned encoder would write past
@@ -135,39 +122,47 @@ Section AlignedEncodeM.
        say about the rest of the .
    *)
 
-  (* Definition EncodeMEquivAlignedEncodeM
+  Definition EncodeMEquivAlignedEncodeM
              (f : EncodeM S ByteString)
              (f' : forall numBytes, AlignedEncodeM numBytes)
-    := forall ce s idx,
-      (padding (fst (f s ce)) = 0 ->
-       forall (v1 : Vector.t char idx) v m v2,
-       exists v',
-         f' _ (Vector.append v1 (Vector.append (n := numBytes (fst (f ce))) (p := m)
-                                               v v2)) idx ce = Some (v', idx + numBytes (fst (f ce)), snd (f ce)) /\
-         ByteString_enqueue_ByteString (build_aligned_ByteString v1)
-                                       (ByteString_enqueue_ByteString (fst (f ce))
-                                                                      (build_aligned_ByteString v2))
-         = build_aligned_ByteString v')%nat
-      /\ (forall numBytes' v, 8 + 8 * numBytes' <= length_ByteString (fst (f ce)) + (8 * idx)
-          -> f' numBytes' v idx ce = None)%nat
-      /\ (forall numBytes' v, padding (fst (f ce)) <> 0 -> f' numBytes' v idx ce = None)%nat.
+    := forall env s idx,
+      (forall t env',
+          f s env = Some (t, env')
+          -> padding t = 0 ->
+          forall (v1 : Vector.t char idx) v m v2,
+          exists v',
+            f' _ (Vector.append v1 (Vector.append (n := numBytes t) (p := m)
+                                                  v v2)) idx s env = Some (v', idx + numBytes t, env') /\
+            ByteString_enqueue_ByteString (build_aligned_ByteString v1)
+                                          (ByteString_enqueue_ByteString t (build_aligned_ByteString v2))
+            = build_aligned_ByteString v')%nat
+      /\ (forall t env' numBytes' v,
+             f s env = Some (t, env')
+             -> 8 + 8 * numBytes' <= length_ByteString t + (8 * idx)
+          -> f' numBytes' v idx s env = None)%nat
+      /\ (forall t env' numBytes' v,
+             f s env = Some (t, env')
+             -> padding t <> 0 -> f' numBytes' v idx s env = None)%nat
+      /\ (forall numBytes' v, f s env = None -> f' numBytes' v idx s env = None).
 
   Lemma EncodeMEquivAlignedEncodeM_trans :
     forall bit_decoder1 byte_decoder1 bit_decoder2 byte_decoder2,
       EncodeMEquivAlignedEncodeM bit_decoder1 byte_decoder1
-      -> (forall ce, bit_decoder1 ce  = bit_decoder2 ce)
+      -> (forall s env, bit_decoder1 s env  = bit_decoder2 s env)
       -> (forall n, AlignedEncodeMEquiv (byte_decoder1 n) (byte_decoder2 n))
       -> EncodeMEquivAlignedEncodeM bit_decoder2 byte_decoder2.
   Proof.
     unfold EncodeMEquivAlignedEncodeM; intros; intuition.
     - revert v1 v v2 H2; rewrite <- ?H0, <- ?H1; intros.
-      destruct (proj1 (H _ _) H2 v1 v m v2); intuition.
+      destruct (proj1 (H _ _ _) _ _ H2 H3 v1 v m v2); intuition.
       eexists; intuition eauto.
       rewrite <- H1; eauto.
     - rewrite <- ?H0, <- ?H1; intros.
-      eapply (proj1 (proj2 (H _ _))); rewrite H0; eauto.
+      eapply (proj1 (proj2 (H _ _ _))); eauto; rewrite H0; eauto.
     - rewrite <- ?H0, <- ?H1; intros.
-      eapply H; rewrite ?H0; eauto.
+      eapply (proj1 (proj2 (proj2 (H _ _ _)))); rewrite ?H0; eauto.
+    - rewrite <- ?H0 in H2.
+      rewrite <- H1; eapply H; eauto.
   Qed.
 
   Local Arguments mult : simpl never.
@@ -175,16 +170,17 @@ Section AlignedEncodeM.
   Definition AlignedEncode_Nil
              numBytes
     : AlignedEncodeM numBytes :=
-    (fun v idx ce => (if idx <? S numBytes then @ReturnAlignedEncodeM _ v idx ce else None)).
+    (fun v idx s env => (if idx <? Datatypes.S numBytes then @ReturnAlignedEncodeM _ v idx s env else None)).
 
   Lemma Return_EncodeMEquivAlignedEncodeM
     : EncodeMEquivAlignedEncodeM
-        (fun (ce : CacheFormat) => (mempty, ce))
+        (fun (s : S) (env : CacheFormat) => Some (mempty, env))
         AlignedEncode_Nil.
   Proof.
     unfold EncodeMEquivAlignedEncodeM, AlignedEncode_Nil, ReturnAlignedEncodeM;
-      intros; simpl in *; intuition.
-    - assert (idx < S (idx + m))%nat as H' by omega;
+      intros; injections; simpl in *; intuition.
+    - injections; simpl.
+      assert (idx < Datatypes.S (idx + m))%nat as H' by omega;
         rewrite <- ltb_lt in H'; rewrite H'.
       revert v.
       eapply Vector.case0; simpl.
@@ -192,77 +188,79 @@ Section AlignedEncodeM.
       pose proof (mempty_left (build_aligned_ByteString v2)) as H'';
         simpl in H'';
       rewrite H'', <- build_aligned_ByteString_append; reflexivity.
-    - destruct (idx <? (S numBytes')) eqn: ?; auto.
-      rewrite ltb_lt in Heqb; omega.
+    - injections; simpl in *.
+      destruct (idx <? (Datatypes.S numBytes')) eqn: ?; auto.
+      rewrite ltb_lt in Heqb.
+      omega.
+    - injections; simpl in *; omega.
+    - discriminate.
   Qed.
 
-  Definition AppendEncodeM
-             {B}
-             (B_Monoid : Monoid B)
-             (encode1 encode2 : EncodeM B)
-    : EncodeM B :=
-    fun ce => let (c, ce') := encode1 ce in
-                let (c', ce') := encode2 ce' in
-                (mappend c c', ce').
+  Local Arguments plus : simpl never.
 
   Lemma Append_EncodeMEquivAlignedEncodeM
-        (encode1 encode2 : EncodeM ByteString)
+        (encode1 encode2 : EncodeM S ByteString)
         (encode1_aligned encode2_aligned : forall {numBytes}, AlignedEncodeM numBytes)
-        (encode1_OK : forall ce, padding (fst (encode1 ce)) = 0)
+        (encode1_OK : forall s env t env',
+            encode1 s env = Some (t, env') -> padding t = 0)
     : EncodeMEquivAlignedEncodeM encode1 (@encode1_aligned)
       -> EncodeMEquivAlignedEncodeM encode2 (@encode2_aligned)
       -> EncodeMEquivAlignedEncodeM
-           (AppendEncodeM _ encode1 encode2)
+           (sequence_Encode encode1 encode2)
            (fun numBytes => AppendAlignedEncodeM encode1_aligned encode2_aligned).
   Proof.
-    unfold EncodeMEquivAlignedEncodeM; intros; specialize (encode1_OK ce); split; intros.
-    - destruct (H ce idx) as [ H' [? ?] ].
-      revert v H' H1 H2 H3;
-        unfold AppendEncodeM;
-        destruct (encode1 ce) as [c' ce'] eqn: ? ;
-        destruct (encode2 ce') eqn: ? ; simpl in *;
-          rewrite numBytes_ByteString_enqueue_ByteString;
-          intros; eauto.
-      destruct (H0 ce' (idx + (numBytes c'))) as [H0' [? ?] ].
-      erewrite <- padding_ByteString_enqueue_aligned_ByteString, Heqp0 in H0'.
-      destruct (H' encode1_OK v1 (fst (Vector_split _ _ v)) _
+    unfold EncodeMEquivAlignedEncodeM; intros; specialize (encode1_OK s env); repeat split; intros.
+    - destruct (H env s idx) as [ H' [? ?] ].
+      revert H1 v H' H2 H3 H4;
+        unfold sequence_Encode;
+        destruct (encode1 s env) as [ [t1 env''] | ] eqn: ? ;
+        [ | intros; try discriminate];
+        simpl; destruct (encode2 s env'') as [ [t2 env'''] | ] eqn: ? ; simpl in *;
+          try (intros; discriminate);
+          intro; injection H1; intros ? ?; subst;
+            simpl; rewrite numBytes_ByteString_enqueue_ByteString;
+              intros; eauto.
+      destruct (H0 env'' s (idx + (numBytes t1))) as [H0' [? [? ?] ] ].
+      specialize (H0' _ _ Heqo0).
+      erewrite <- padding_ByteString_enqueue_aligned_ByteString in H0'.
+      destruct (H' _ _ (eq_refl _) (encode1_OK _ _ (eq_refl _)) v1 (fst (Vector_split _ _ v)) _
                    (Vector.append (snd (Vector_split _ _ v)) v2)) as [? [? ?] ].
-      assert (idx + (numBytes c' + (numBytes b + m)) =
-              (idx + numBytes c') + (numBytes b + m)) by omega; simpl in *.
-      destruct (H0' H1 (fst (Vector_split _ _ (eq_rect _ (Vector.t char) x _ H8)))
-                    (fst (Vector_split _ _ (snd (Vector_split _ _ (eq_rect _ (Vector.t char) x _ H8)))))
-                    _ (snd (Vector_split _ _ (snd (Vector_split _ _ (eq_rect _ (Vector.t char) x _ H8)))))
+      assert (idx + (numBytes t1 + (numBytes t2 + m)) =
+              (idx + numBytes t1) + (numBytes t2 + m)) by omega; simpl in *.
+      destruct (H0' H2 (fst (Vector_split _ _ (eq_rect _ (Vector.t char) x _ H10)))
+                    (fst (Vector_split _ _ (snd (Vector_split _ _ (eq_rect _ (Vector.t char) x _ H10)))))
+                    _ (snd (Vector_split _ _ (snd (Vector_split _ _ (eq_rect _ (Vector.t char) x _ H10)))))
                ).
-      assert (idx + numBytes c' + (numBytes b + m) =
-              idx + (numBytes c' + numBytes b + m)) as H11 by omega.
-      assert (idx + (numBytes c' + (numBytes b + m)) =
-              (idx + (numBytes c' + numBytes b + m))) by omega; simpl in *.
+      assert (idx + numBytes t1 + (numBytes t2 + m) =
+              idx + (numBytes t1 + numBytes t2 + m)) as H11' by omega.
+      assert (idx + (numBytes t1 + (numBytes t2 + m)) =
+              (idx + (numBytes t1 + numBytes t2 + m))) by omega; simpl in *.
       unfold AppendAlignedEncodeM.
-      replace (encode1_aligned (idx + ((numBytes c' + numBytes b) + m))
-                               (Vector.append v1 (Vector.append v v2)) idx ce)
-        with (Some (eq_rect _ (Vector.t char) x _ H10, idx + numBytes c', ce'));
+      replace (encode1_aligned (idx + ((numBytes t1 + numBytes t2) + m))
+                               (Vector.append v1 (Vector.append v v2)) idx s env)
+        with (Some (eq_rect _ (Vector.t char) x _ H12, idx + numBytes t1, env''));
         simpl.
-      + revert H10; rewrite <- H11; intros.
-        rewrite (plus_assoc idx (numBytes c') (numBytes b)).
+      + revert H12; rewrite <- H11'; intros.
+        rewrite (plus_assoc idx (numBytes t1) (numBytes t2)).
         eexists _; intuition.
-        * etransitivity; [ | apply H12].
+        * etransitivity; [ | apply H4].
           f_equal.
           rewrite <- !Vector_split_append.
           f_equal; eapply UIP_dec; intros; decide equality.
-        * rewrite <- H13.
+        * rewrite <- H15.
           rewrite ByteString_enqueue_ByteString_assoc.
           rewrite ByteString_enqueue_ByteString_assoc.
           rewrite <- ByteString_enqueue_ByteString_assoc.
-          symmetry in H7; destruct (build_aligned_ByteString_split' _ _ _ H7)
-            as [? H']; symmetry in H'; destruct (build_aligned_ByteString_split _ _ _ H').
-          revert H14 H7; clear.
+          symmetry in H9; destruct (build_aligned_ByteString_split' _ _ _ H9)
+            as [? H'']; symmetry in H''; destruct (build_aligned_ByteString_split _ _ _ H'').
+          revert H16 H9; clear.
           intro.
-          revert H8 x v.
-          assert (idx + (numBytes c' + (numBytes b + m)) - idx - (numBytes b + m) = numBytes c')
-            as H'' by omega; revert x2 H14; rewrite H''; clear H''.
-          generalize (numBytes c'); intros; subst.
-          rewrite <- !build_aligned_ByteString_append in H7;
-            apply build_aligned_ByteString_inj in H7; subst.
+          revert H10 x v.
+          assert (idx + (numBytes t1 + (numBytes t2 + m)) - idx - (numBytes t2 + m) = numBytes t1)
+            as H''' by omega; revert x2 H16; rewrite H'''; clear H'''.
+          generalize (numBytes t1); intros; subst.
+          rewrite <- !build_aligned_ByteString_append in H9;
+            apply build_aligned_ByteString_inj in H9; subst.
           rewrite <- !build_aligned_ByteString_append; repeat f_equal.
           erewrite Vector_append_assoc.
           rewrite <- Equality.transport_pp.
@@ -272,136 +270,165 @@ Section AlignedEncodeM.
           rewrite <- Equality.transport_pp.
           erewrite (UIP_dec _ _ (eq_refl _)); simpl.
           rewrite <- !Vector_append_split_snd; reflexivity.
-      + generalize x H6 H10; clear; intros.
+      + generalize x H8 H12; clear; intros.
          replace (Some
-                    (eq_rect (idx + (numBytes c' + (numBytes b + m)))
-                             (Vector.t char) x (idx + (numBytes c' + numBytes b + m)) H10,
-                     idx + numBytes c', ce')) with
-             (eq_rect _ (fun x => option ((Vector.t char x) * nat * CacheFormat))%type (Some (x, idx + numBytes c', ce')) _ H10).
-         rewrite <- H6.
-         assert (idx + (numBytes c' + numBytes b + m) =
-                 idx + (numBytes c' + (numBytes b + m))) by omega.
-         replace (Vector.append v1 (Vector.append (fst (Vector_split (numBytes c') (numBytes b) v))
-                                                  (Vector.append (snd (Vector_split (numBytes c') (numBytes b) v)) v2)))
+                    (eq_rect (idx + (numBytes t1 + (numBytes t2 + m)))
+                             (Vector.t char) x (idx + (numBytes t1 + numBytes t2 + m)) H12,
+                     idx + numBytes t1, env'')) with
+             (eq_rect _ (fun x => option ((Vector.t char x) * nat * CacheFormat))%type (Some (x, idx + numBytes t1, env'')) _ H12).
+         rewrite <- H8.
+         assert (idx + (numBytes t1 + numBytes t2 + m) =
+                 idx + (numBytes t1 + (numBytes t2 + m))) by omega.
+         replace (Vector.append v1 (Vector.append (fst (Vector_split (numBytes t1) (numBytes t2) v))
+                                                  (Vector.append (snd (Vector_split (numBytes t1) (numBytes t2) v)) v2)))
            with (eq_rect _ (Vector.t char) (Vector.append v1 (Vector.append v v2)) _ H).
          assert (forall n m (H' : n = m) (v : Vector.t char n),
-                    encode1_aligned m (eq_rect n (Vector.t char) v _ H') idx ce =
+                    encode1_aligned m (eq_rect n (Vector.t char) v _ H') idx s env =
                     eq_rect n (fun x => option ((Vector.t char x) * nat * CacheFormat))%type
-                            (encode1_aligned _ v idx ce) _ H') as H'
+                            (encode1_aligned _ v idx s env) _ H') as H'
              by (intros ? ? H'; rewrite H'; reflexivity).
          rewrite H', <- Equality.transport_pp.
          erewrite (UIP_dec _ _ (eq_refl _)); reflexivity.
-         assert (numBytes c' + numBytes b + m = numBytes c' + (numBytes b + m)) by omega.
-         replace (Vector.append (fst (Vector_split (numBytes c') (numBytes b) v))
-                                (Vector.append (snd (Vector_split (numBytes c') (numBytes b) v)) v2))
+         assert (numBytes t1 + numBytes t2 + m = numBytes t1 + (numBytes t2 + m)) by omega.
+         replace (Vector.append (fst (Vector_split (numBytes t1) (numBytes t2) v))
+                                (Vector.append (snd (Vector_split (numBytes t1) (numBytes t2) v)) v2))
            with (eq_rect _ (Vector.t char) (Vector.append v v2) _ H0)
            by (erewrite Vector_append_assoc, <- Vector_split_append; reflexivity).
          erewrite Vector_append_assoc', Vector_append_assoc, <- Equality.transport_pp.
          reflexivity.
-         destruct H10; reflexivity.
-      + apply encode1_OK.
-    - specialize (H ce idx);
-        unfold AppendEncodeM;
-        destruct (encode1 ce) as [c' ce'] eqn: ? ;
-        destruct (encode2 ce') eqn: ? ; simpl in *; split; intros.
-      + pose proof (proj1 H encode1_OK ).
-        rewrite length_ByteString_enqueue_ByteString in H1.
-        unfold AppendAlignedEncodeM; destruct (encode1_aligned numBytes' v idx ce) eqn: ? ;
+         destruct H12; reflexivity.
+      + eapply encode1_OK; eauto.
+    - specialize (H env s idx);
+        unfold sequence_Encode in *;
+        destruct (encode1 s env) as [ [t1 env''] | ] eqn: ? ;
+        simpl in *; [ | intros; try discriminate];
+        simpl; destruct (encode2 s env'') as [ [t2 env'''] | ] eqn: ? ; simpl in *;
+          try (intros; discriminate).
+      pose proof (proj1 H _ _ (eq_refl _) (encode1_OK _ _ (eq_refl _))).
+      injections.
+      rewrite length_ByteString_enqueue_ByteString in H2.
+      unfold AppendAlignedEncodeM; destruct (encode1_aligned numBytes' v idx s env) eqn: ? ;
           simpl; eauto.
         destruct (le_lt_dec (8 + 8 * numBytes')
-                            (length_ByteString c' + 8 * idx)).
-        { eauto; simpl in l; eapply (proj1 (proj2 H)) in l; rewrite l in Heqo; discriminate. }
+                            (length_ByteString t1 + 8 * idx)).
+        { eauto; simpl in l; eapply (proj1 (proj2 H)) in l; eauto; rewrite Heqo1 in l; discriminate. }
         rewrite length_ByteString_no_padding in l by eauto.
-        pose proof (proj1 (proj2 (H0 ce' (snd (fst p))))) as H'.
-        assert (numBytes c' + idx < S numBytes')%nat by omega; clear l.
-        assert (idx + numBytes c' <= numBytes')%nat by omega.
+        pose proof (proj1 (proj2 (H0 env'' s (snd (fst p))))) as H'.
+        assert (numBytes t1 + idx < Datatypes.S numBytes')%nat by omega; clear l.
+        assert (idx + numBytes t1 <= numBytes')%nat by omega.
         destruct (Vector_split_lt _ _ H4 v) as [? [? [? [? ?] ] ] ].
         pose proof (proj1 (proj2 (H))) as H'' .
-        destruct (H2 (fst (Vector_split _ _ x0)) (snd (Vector_split _ _ x0)) _ x1) as [v' [? ?] ].
+        destruct (H3 (fst (Vector_split _ _ x0)) (snd (Vector_split _ _ x0)) _ x1) as [v' [? ?] ].
         erewrite <- H'; f_equal; clear H'.
-        * revert p Heqo H6.
-          rewrite H5.
-          rewrite <- x2; simpl; clear.
-          rewrite Vector_append_assoc with (H := sym_eq (plus_assoc idx (numBytes c') x)), <- Vector_split_append.
-          generalize v' (eq_sym (plus_assoc idx (numBytes c') x)).
-          rewrite (plus_assoc idx (numBytes c') x).
-          intros. erewrite (UIP_dec _ _ (eq_refl _)) in H6; simpl in H6.
-          rewrite Heqo in H6; destruct p as [ [? ?] ?]; simpl in *; congruence.
-        * rewrite Heqp0; simpl.
-          replace (8 * snd (fst p)) with (length_ByteString c' + 8 * idx); try omega.
-          rewrite length_ByteString_no_padding by eauto.
-          revert p Heqo H6.
-          rewrite H5.
-          rewrite <- x2; simpl; clear.
-          rewrite Vector_append_assoc with (H := sym_eq (plus_assoc idx (numBytes c') x)), <- Vector_split_append.
-          generalize v' (eq_sym (plus_assoc idx (numBytes c') x)).
-          rewrite (plus_assoc idx (numBytes c') x).
-          intros. erewrite (UIP_dec _ _ (eq_refl _)) in H6; simpl in H6.
-          rewrite Heqo in H6; destruct p as [ [? ?] ?]; simpl in *; injections.
-          omega.
-      + pose proof (proj1 H encode1_OK ).
-        rewrite padding_ByteString_enqueue_aligned_ByteString in H1 by eauto.
-        unfold AppendAlignedEncodeM; destruct (encode1_aligned numBytes' v idx ce) eqn: ? ;
+      + revert p Heqo1 H6.
+        rewrite H5.
+        rewrite <- x2; simpl; clear.
+        rewrite Vector_append_assoc with (H := sym_eq (plus_assoc idx (numBytes t1) x)), <- Vector_split_append.
+        generalize v' (eq_sym (plus_assoc idx (numBytes t1) x)).
+        rewrite (plus_assoc idx (numBytes t1) x).
+        intros. erewrite (UIP_dec _ _ (eq_refl _)) in H6; simpl in H6.
+        rewrite Heqo1 in H6; destruct p as [ [? ?] ?]; simpl in *; congruence.
+      + rewrite Heqo0; simpl; eauto.
+      + replace (8 * snd (fst p)) with (length_ByteString t1 + 8 * idx); try omega.
+        rewrite length_ByteString_no_padding by eauto.
+        revert p Heqo1 H6.
+        rewrite H5.
+        rewrite <- x2; simpl; clear.
+        rewrite Vector_append_assoc with (H := sym_eq (plus_assoc idx (numBytes t1) x)), <- Vector_split_append.
+        generalize v' (eq_sym (plus_assoc idx (numBytes t1) x)).
+        rewrite (plus_assoc idx (numBytes t1) x).
+        intros. erewrite (UIP_dec _ _ (eq_refl _)) in H6; simpl in H6.
+        rewrite Heqo1 in H6; destruct p as [ [? ?] ?]; simpl in *; injections.
+        omega.
+      - specialize (H env s idx);
+        unfold sequence_Encode in *;
+        destruct (encode1 s env) as [ [t1 env''] | ] eqn: ? ;
+        simpl in *; [ | intros; try discriminate];
+        simpl; destruct (encode2 s env'') as [ [t2 env'''] | ] eqn: ? ; simpl in *;
+          try (intros; discriminate); injections.
+        pose proof (proj1 H _ _ (eq_refl _) (encode1_OK _ _ (eq_refl _))).
+        rewrite padding_ByteString_enqueue_aligned_ByteString in H2 by eauto.
+        unfold AppendAlignedEncodeM; destruct (encode1_aligned numBytes' v idx s env) eqn: ? ;
           simpl; eauto.
         destruct (le_lt_dec (8 + 8 * numBytes')
-                            (length_ByteString c' + 8 * idx)).
-        { eauto; simpl in l; eapply (proj1 (proj2 H)) in l; rewrite l in Heqo; discriminate. }
+                            (length_ByteString t1 + 8 * idx)).
+        { eauto; simpl in l; eapply (proj1 (proj2 H)) in l; eauto; rewrite l in Heqo1; discriminate. }
         rewrite length_ByteString_no_padding in l by eauto.
-        pose proof (proj2 (proj2 (H0 ce' (snd (fst p))))) as H'.
-        assert (numBytes c' + idx < S numBytes')%nat by omega; clear l.
-        assert (idx + numBytes c' <= numBytes')%nat by omega.
+        pose proof (proj1 (proj2 (proj2 (H0 env'' s (snd (fst p)))))) as H'.
+        assert (numBytes t1 + idx < Datatypes.S numBytes')%nat by omega; clear l.
+        assert (idx + numBytes t1 <= numBytes')%nat by omega.
         destruct (Vector_split_lt _ _ H4 v) as [? [? [? [? ?] ] ] ].
         pose proof (proj2 (proj2 (H))) as H'' .
-        destruct (H2 (fst (Vector_split _ _ x0)) (snd (Vector_split _ _ x0)) _ x1) as [v' [? ?] ].
-        erewrite <- H'; f_equal; clear H'.
-        * revert p Heqo H6.
+        destruct (H1 (fst (Vector_split _ _ x0)) (snd (Vector_split _ _ x0)) _ x1) as [v' [? ?] ].
+        erewrite <- H'; f_equal; clear H'; eauto.
+        * revert p Heqo1 H6.
           rewrite H5.
           rewrite <- x2; simpl; clear.
-          rewrite Vector_append_assoc with (H := sym_eq (plus_assoc idx (numBytes c') x)), <- Vector_split_append.
-          generalize v' (eq_sym (plus_assoc idx (numBytes c') x)).
-          rewrite (plus_assoc idx (numBytes c') x).
+          rewrite Vector_append_assoc with (H := sym_eq (plus_assoc idx (numBytes t1) x)), <- Vector_split_append.
+          generalize v' (eq_sym (plus_assoc idx (numBytes t1) x)).
+          rewrite (plus_assoc idx (numBytes t1) x).
           intros. erewrite (UIP_dec _ _ (eq_refl _)) in H6; simpl in H6.
-          rewrite Heqo in H6; destruct p as [ [? ?] ?]; simpl in *; congruence.
-        * rewrite Heqp0; simpl.
-          replace (8 * snd (fst p)) with (length_ByteString c' + 8 * idx); try omega.
-          rewrite !length_ByteString_no_padding; eauto.
-          revert p Heqo H6.
-          rewrite H5.
-          rewrite <- x2; simpl; clear.
-          rewrite Vector_append_assoc with (H := sym_eq (plus_assoc idx (numBytes c') x)), <- Vector_split_append.
-          generalize v' (eq_sym (plus_assoc idx (numBytes c') x)).
-          rewrite (plus_assoc idx (numBytes c') x).
-          intros. erewrite (UIP_dec _ _ (eq_refl _)) in H6; simpl in H6.
-          rewrite Heqo in H6; destruct p as [ [? ?] ?]; simpl in *; injections.
+          rewrite Heqo1 in H6; destruct p as [ [? ?] ?]; simpl in *; try congruence.
+      - specialize (H env s idx);
+        unfold sequence_Encode in *;
+        destruct (encode1 s env) as [ [t1 env''] | ] eqn: ? ; simpl in *.
+        + destruct (encode2 s env'') as [ [t2 env'''] | ] eqn: ? ; simpl in *;
+             try discriminate.
+          unfold AppendAlignedEncodeM.
+          destruct (Nat.le_decidable (8 + 8 * numBytes') (length_ByteString t1 + 8 * idx)).
+          erewrite (proj1 (proj2 H)); eauto.
+          destruct (PeanoNat.Nat.eq_dec (padding t1) 0).
+          unfold length_ByteString in H2; rewrite e in H2; simpl in H2.
+          assert (exists m, numBytes' = idx + (numBytes t1 + m)).
+          exists (numBytes' - (idx + numBytes t1)).
           omega.
-      Grab Existential Variables.
-      decide equality.
-      decide equality.
-      decide equality.
-      decide equality.
-      omega.
-      decide equality.
-      decide equality.
-      omega.
-      decide equality.
-      omega.
+          destruct H3.
+          pose proof (proj1 H _ _ (eq_refl _) (encode1_OK _ _ (eq_refl _))) as H'.
+          destruct (H' (fst (Vector_split _ _ (eq_rect _ _ v _ H3)))
+                         (fst (Vector_split _ _ (snd (Vector_split _ _ (eq_rect _ _ v _ H3)))))
+                         _
+                         (snd (Vector_split _ _ (snd (Vector_split _ _ (eq_rect _ _ v _ H3))))))
+            as [v' [? ?] ].
+          replace (encode1_aligned _ v idx s env)
+            with (Some (eq_rect _ (Vector.t char) v' _ (sym_eq H3), idx + numBytes t1, env'')).
+          * simpl; eapply H0; rewrite <- Heqo0; f_equal.
+          * generalize v' H3 H4; clear; intros.
+            revert v v' H4; rewrite H3; intros; simpl; f_equal.
+            rewrite <- H4; f_equal.
+            rewrite <- !Vector_split_append; reflexivity.
+          * erewrite (proj1 (proj2 (proj2 H))); eauto.
+        + unfold AppendAlignedEncodeM; rewrite (proj2 (proj2 (proj2 H))); simpl; eauto.
+          Grab Existential Variables.
+          decide equality.
+          decide equality.
+          decide equality.
+          omega.
+          decide equality.
+          decide equality.
+          omega.
+          decide equality.
+          omega.
   Qed.
 
   Definition CorrectAlignedEncoder
-             (format : CacheFormat -> Comp (ByteString * CacheFormat))
+             (format : FormatM S ByteString)
              (encoder : forall sz, AlignedEncodeM sz)
-    := {encoder' : _ &
-                   (forall ce, refine (format ce) (ret (encoder' ce)))
-                   /\ (forall ce, padding (fst (encoder' ce)) = 0)
+    := {encoder' : EncodeM S ByteString &
+                   (forall s env t env',
+                       encoder' s env = Some (t, env')
+                       -> refine (format s env) (ret (t, env')))
+                   /\ (forall s env t env',
+                          encoder' s env = Some (t, env')
+                       -> padding t = 0)
                    /\ EncodeMEquivAlignedEncodeM encoder' encoder}.
 
   Lemma CorrectAlignedEncoderForDoneC
-    : CorrectAlignedEncoder (fun e => Return (ByteString_id, e)) AlignedEncode_Nil.
+    : CorrectAlignedEncoder (fun s e => Return (ByteString_id, e)) AlignedEncode_Nil.
   Proof.
     unfold CorrectAlignedEncoder; intros.
-    eexists _; split; [ | split].
-    intros; higher_order_reflexivity.
-    reflexivity.
+    eexists (fun _ env => Some (ByteString_id, env)); split; [ | split]; intros.
+    congruence.
+    injections; reflexivity.
     eapply Return_EncodeMEquivAlignedEncodeM.
   Qed.
 
@@ -426,13 +453,13 @@ Section AlignedEncodeM.
   Qed. *)
 
   Lemma CorrectAlignedEncoderForThenC
-        (format_A format_B : CacheFormat -> Comp (ByteString * CacheFormat))
+        (format_A format_B : FormatM S ByteString)
         (encode_A : forall sz, AlignedEncodeM sz)
         (encode_B : forall sz, AlignedEncodeM sz)
         (encoder_A_OK : CorrectAlignedEncoder format_A encode_A)
         (encoder_B_OK : CorrectAlignedEncoder format_B encode_B)
     : CorrectAlignedEncoder
-        (format_B ThenC format_A)
+        (format_B ++ format_A)
         (fun sz => AppendAlignedEncodeM (encode_B sz) (encode_A sz)).
   Proof.
     unfold CorrectAlignedEncoder; intros.
@@ -442,44 +469,56 @@ Section AlignedEncodeM.
     4: apply H5.
     4: apply H4.
     3: apply H0.
-    unfold compose, Bind2.
+    unfold sequence_Format, sequence_Encode, Bind2 in *.
+    apply_in_hyp DecodeBindOpt_inv; destruct_ex; split_and.
+    symmetry in H7.
+    apply_in_hyp DecodeBindOpt_inv; destruct_ex; split_and.
+    injections.
+    specialize (H _ _ _ _ H7).
+    specialize (H3 _ _ _ _ H7).
+    specialize (H1 _ _ _ _ H6).
+    specialize (H0 _ _ _ _ H6).
     rewrite H1, Monad.refineEquiv_bind_unit.
     rewrite H, Monad.refineEquiv_bind_unit.
-    simpl; unfold AppendEncodeM.
-    destruct (encoder_B ce); simpl;
-      destruct (encoder_A c); simpl; reflexivity.
-    simpl; unfold AppendEncodeM.
-    specialize (H0 ce); destruct (encoder_B ce); simpl.
-    specialize (H3 c); destruct (encoder_A c); simpl.
-    simpl in *.
+    reflexivity.
+    unfold sequence_Format, sequence_Encode, Bind2 in *.
+    apply_in_hyp DecodeBindOpt_inv; destruct_ex; split_and.
+    symmetry in H7.
+    apply_in_hyp DecodeBindOpt_inv; destruct_ex; split_and.
+    injections.
     rewrite padding_ByteString_enqueue_aligned_ByteString; eauto.
   Qed.
 
 End AlignedEncodeM.
 
-Lemma refine_CorrectAlignedEncoder {cache : Cache}
+Lemma refine_CorrectAlignedEncoder
+      {S : Type}
+      {cache : Cache}
   : forall format format' encode,
-    (forall ce : CacheFormat, refine (format ce) (format' ce))
+    (forall (s : S) (env : CacheFormat),
+        refine (format s env) (format' s env))
     -> (CorrectAlignedEncoder format' encode)
     -> (CorrectAlignedEncoder format encode).
 Proof.
   unfold CorrectAlignedEncoder; intros.
-  destruct X; eexists; intuition.
-  - rewrite H; eauto.
+  destruct X as [? [? ?] ]; eexists; intuition eauto.
+  rewrite H; eauto.
 Qed.
 
-Lemma CorrectAlignedEncoderThenCAssoc {cache : Cache}
-      (format_A format_B format_C : CacheFormat -> Comp (ByteString * CacheFormat))
+Lemma CorrectAlignedEncoderThenCAssoc
+      {S : Type}
+      {cache : Cache}
+      (format_A format_B format_C : FormatM S ByteString)
       (encode : forall sz, AlignedEncodeM sz)
   : CorrectAlignedEncoder
-      ((format_A ThenC format_B) ThenC format_C)
+      ((format_A ++ format_B) ++ format_C)
       encode
     -> CorrectAlignedEncoder
-         (format_A ThenC format_B ThenC format_C)
+         (format_A ++ format_B ++ format_C)
          encode.
 Proof.
   intros; eapply refine_CorrectAlignedEncoder; eauto.
-  unfold compose; intros.
+  unfold sequence_Format; intros.
   unfold Bind2.
   repeat setoid_rewrite Monad.refineEquiv_bind_bind.
   setoid_rewrite Monad.refineEquiv_bind_unit; simpl; f_equiv; intro.
@@ -488,33 +527,37 @@ Proof.
   rewrite ByteString_enqueue_ByteString_assoc; reflexivity.
 Qed.
 
-Corollary Guarded_CorrectAlignedEncoderThenCAssoc {cache : Cache}
-          (format_A format_B format_C : CacheFormat -> Comp (ByteString * CacheFormat))
+Corollary Guarded_CorrectAlignedEncoderThenCAssoc
+          {S : Type}
+          {cache : Cache}
+          (format_A format_B format_C : FormatM S ByteString)
           (encode : forall sz, AlignedEncodeM sz)
-  : (forall ce bs ce', computes_to (format_A ce) (bs, ce') ->
+  : (forall env s bs env', computes_to (format_A s env) (bs, env') ->
                        length_ByteString bs < 8)%nat
     -> CorrectAlignedEncoder
-         ((format_A ThenC format_B) ThenC format_C)
+         ((format_A ++ format_B) ++ format_C)
          encode
     -> CorrectAlignedEncoder
-         (format_A ThenC format_B ThenC format_C)
+         (format_A ++ format_B ++ format_C)
          encode.
 Proof.
   intros; eapply CorrectAlignedEncoderThenCAssoc; eauto.
 Qed.
 
-Lemma CorrectAlignedEncoderThenCAssoc' {cache : Cache}
-      (format_A format_B format_C : CacheFormat -> Comp (ByteString * CacheFormat))
+Lemma CorrectAlignedEncoderThenCAssoc'
+      {S : Type}
+      {cache : Cache}
+      (format_A format_B format_C : FormatM S ByteString)
       (encode : forall sz, AlignedEncodeM sz)
   : CorrectAlignedEncoder
-      (format_A ThenC format_B ThenC format_C)
+      (format_A ++ format_B ++ format_C)
       encode
     -> CorrectAlignedEncoder
-         ((format_A ThenC format_B) ThenC format_C)
+         ((format_A ++ format_B) ++ format_C)
          encode.
 Proof.
   intros; eapply refine_CorrectAlignedEncoder; eauto.
-  unfold compose; intros.
+  unfold sequence_Format; intros.
   unfold Bind2.
   repeat setoid_rewrite Monad.refineEquiv_bind_bind.
   setoid_rewrite Monad.refineEquiv_bind_unit; simpl; f_equiv; intro.
@@ -529,17 +572,29 @@ Definition Format_Source_Intersection
            (format : @FormatM A B cache)
            (predicate : A -> Prop)
   : @FormatM A B cache
-  := fun a ce bce =>
+  := fun a env benv =>
        predicate a /\
-       format a ce bce.
+       format a env benv.
 
-Definition CorrectAlignedEncoderFor {A} {cache}
-           (format : @FormatM A ByteString cache)
-           (predicate : A -> Prop)
-  := {encode : _ & forall a,
-          predicate a ->
-          CorrectAlignedEncoder (format a) (encode a)}.
+Definition CorrectAlignedEncoderFor {S} {cache}
+           (format : @FormatM S ByteString cache)
+  := {encode : _ & CorrectAlignedEncoder format encode}.
+
+Definition SetCurrentByte (* Sets a single byte at the current index and increments the current index. *)
+           {cache : Cache}
+           {cacheAddNat : CacheAdd cache nat}
+           {n : nat}
+  : @AlignedEncodeM cache char n :=
+  fun v idx s ce => if (idx <? n) then Some (set_nth' v idx s, Datatypes.S idx, addE ce 8) else None.
+
+Definition SetByteAt (* Sets the bytes at the specified index and sets the current index
+                        to the following position. *)
+           {cache : Cache}
+           {cacheAddNat : CacheAdd cache nat}
+           {n : nat}
+           (idx' : nat)
+  : AlignedEncodeM n :=
+  fun v idx s ce => if (NPeano.ltb idx' n) then Some (set_nth' v idx' s, Datatypes.S idx', addE ce 8) else None.
 
 Delimit Scope AlignedEncodeM_scope with AlignedEncodeM.
-Notation "y >> z" := (AppendAlignedEncodeM y z) : AlignedEncodeM_scope. *)
-End AlignedEncodeM.
+Notation "y >> z" := (AppendAlignedEncodeM y z) : AlignedEncodeM_scope.
