src/Narcissus/Formats/NatOpt.v
@@ -1,5 +1,7 @@
 Require Import
         Fiat.Narcissus.Common.Specs
+        Fiat.Narcissus.BaseFormats
+        Fiat.Narcissus.Formats.Bool
         Fiat.Narcissus.Formats.WordOpt.
 Require Import
         Coq.omega.Omega
@@ -8,17 +10,38 @@ Require Import
 Section Nat.
   Variable sz : nat.
 
-  Context {B : Type}.
+  Context {T : Type}.
   Context {cache : Cache}.
   Context {cacheAddNat : CacheAdd cache nat}.
-  Context {monoid : Monoid B}.
+  Context {monoid : Monoid T}.
   Context {monoidUnit : QueueMonoidOpt monoid bool}.
 
   Definition format_nat (n : nat) (ce : CacheFormat)
-    : Comp (B * CacheFormat) :=
+    : Comp (T * CacheFormat) :=
     format_word (natToWord sz n) ce.
 
-  Definition encode_nat (n : nat) (ce : CacheFormat) : B * CacheFormat :=
+  Open Scope vector_scope.
+  Definition format_nat'
+    : FormatM nat T :=
+    Fix_Format
+      (fun rec : FormatM nat T =>
+         Union_Format [(fun (_ : unit) s => s = 0) <$> StrictTerminal_Format;
+                         (fun n' s => s = S n') <$> Projection_Format (fun n' => Nat.eqb (n' mod 2) 1) format_bool
+                                                ++ rec]%format).
+
+  Theorem Nat_decode_correct 
+    : {decode_nat : _ &
+                     CorrectDecoder_simpl format_nat' decode_nat}.
+  Proof.
+    eexists; unfold format_nat'; intros.
+    eapply CorrectDecoder_Fix; intros.
+    - unfold Frame.monotonic_function; simpl; intros.
+      admit.
+    - 
+  Abort.
+
+
+  Definition encode_nat (n : nat) (ce : CacheFormat) : T * CacheFormat :=
     encode_word (natToWord sz n) ce.
 
   Lemma refine_format_nat :
@@ -28,7 +51,7 @@ Section Nat.
     reflexivity.
   Qed.
 
-  Definition decode_nat (b : B) (cd : CacheDecode) : option (nat * B * CacheDecode) :=
+  Definition decode_nat (b : T) (cd : CacheDecode) : option (nat * T * CacheDecode) :=
     `(w, b, cd) <- decode_word (sz:=sz) b cd;
       Some (wordToNat w, b, cd).
 
