src/Narcissus/Formats/WordOpt.v
@@ -3,29 +3,27 @@ Require Import
         Fiat.Common
         Fiat.Computation.Notations
         Fiat.Narcissus.Common.Specs
-        Fiat.Narcissus.Common.WordFacts.
+        Fiat.Narcissus.Common.WordFacts
+        Fiat.Narcissus.BaseFormats.
 
-Unset Implicit Arguments.
 Section Word.
   Context {sz : nat}.
 
-  Context {B : Type}.
+  Context {T : Type}.
   Context {cache : Cache}.
   Context {cacheAddNat : CacheAdd cache nat}.
-  Context {monoid : Monoid B}.
+  Context {monoid : Monoid T}.
   Context {monoidUnit : QueueMonoidOpt monoid bool}.
 
-  Fixpoint encode_word' (s : nat) (w : word s) (b' : B) : B :=
+  Fixpoint encode_word' (s : nat) (w : word s) (b' : T) : T :=
     match w with
     | WO => b'
     | WS b s' w' => enqueue_opt b (encode_word' s' w' b')
     end.
 
-  Eval compute in (wordToNat (WS true (WS false (WS false (WS false (WO)))))).
+  Definition encode_word (w : word sz) (ce : CacheFormat) : T * CacheFormat := (encode_word' sz w mempty, addE ce sz).
 
-  Definition encode_word (w : word sz) (ce : CacheFormat) : B * CacheFormat := (encode_word' sz w mempty, addE ce sz).
-
-  Definition format_word (w : word sz) (ce : CacheFormat) : Comp (B * CacheFormat) :=
+  Definition format_word (w : word sz) (ce : CacheFormat) : Comp (T * CacheFormat) :=
     ret (encode_word' sz w mempty, addE ce sz).
 
   Fixpoint SW_word {sz} (b : bool) (w : word sz) : word (S sz) :=
@@ -58,7 +56,7 @@ Section Word.
       rewrite (IHn x0) at 1; reflexivity.
   Qed.
 
-  Fixpoint decode_word' (s : nat) (b : B) {struct s} : option (word s * B) :=
+  Fixpoint decode_word' (s : nat) (b : T) {struct s} : option (word s * T) :=
     match s with
     | O => Some (WO, b)
     | S s' =>
@@ -67,7 +65,7 @@ Section Word.
       Some (SW_word c w', b')
     end.
 
-  Definition decode_word (b : B) (cd : CacheDecode) : option (word sz * B * CacheDecode) :=
+  Definition decode_word (b : T) (cd : CacheDecode) : option (word sz * T * CacheDecode) :=
     Ifopt decode_word' sz b as decoded Then Some (decoded, addD cd sz) Else None.
 
   Lemma enqueue_opt_format_word :
@@ -166,7 +164,7 @@ Section Word.
       rewrite mempty_left; auto.
     - destruct (dequeue_opt bin) as [ [? ?] | ] eqn: ? ;
         simpl in *; try discriminate.
-      destruct (decode_word' sz0 b0) as [ [? ?] | ] eqn: ? ;
+      destruct (decode_word' sz0 t) as [ [? ?] | ] eqn: ? ;
         simpl in *; try discriminate.
       injections.
       apply IHsz0 in Heqo0; subst.
@@ -203,7 +201,7 @@ Section Word.
   Qed.
 
   Lemma decode_word'_le
-    : forall (a : word sz) (b' b1 : B),
+    : forall (a : word sz) (b' b1 : T),
       decode_word' _ b1 = Some (a, b') -> le_B b' b1.
   Proof.
     intros; apply decode_encode_word'_Some in H; subst.
@@ -212,8 +210,8 @@ Section Word.
   Qed.
 
   Lemma decode_word_le
-    : forall (b1 : B) (cd : CacheDecode) (a : word sz)
-             (b' : B) (cd' : CacheDecode),
+    : forall (b1 : T) (cd : CacheDecode) (a : word sz)
+             (b' : T) (cd' : CacheDecode),
       decode_word b1 cd = Some (a, b', cd') -> le_B b' b1.
   Proof.
     unfold decode_word.
@@ -224,14 +222,14 @@ Section Word.
   Qed.
 
   Lemma decode_word'_lt
-    : forall (a : word (S sz)) (b' b1 : B),
+    : forall (a : word (S sz)) (b' b1 : T),
       decode_word' _ b1 = Some (a, b') -> lt_B b' b1.
   Proof.
     simpl; intros; injections; unfold lt_B.
     destruct (dequeue_opt b1) as [ [? ?] | ] eqn: ? ;
       subst; simpl in *; try discriminate.
     apply measure_dequeue_Some in Heqo; subst.
-    destruct (decode_word' sz b0) as [ [? ?] | ] eqn: ? ;
+    destruct (decode_word' sz t) as [ [? ?] | ] eqn: ? ;
         subst; simpl in *; try discriminate.
     eapply decode_word'_le in Heqo0; injections.
     rewrite Heqo.
@@ -241,8 +239,8 @@ Section Word.
   Qed.
 
   Lemma decode_word_lt
-    : forall (b' : B) (cd : CacheDecode) (a : word (S sz))
-             (b1 : B) (cd' : CacheDecode),
+    : forall (b' : T) (cd : CacheDecode) (a : word (S sz))
+             (b1 : T) (cd' : CacheDecode),
       Ifopt decode_word' _ b' as decoded Then Some (decoded, addD cd (S sz)) Else None = Some (a, b1, cd') -> lt_B b1 b'.
   Proof.
     intros; destruct (decode_word' (S sz) b') as [ [? ?] | ] eqn: ? ;
@@ -262,11 +260,11 @@ Section Word.
              (sz : nat) :=
     format_unused_word' sz mempty tt.
 
-  Fixpoint monoid_get_word {B}
-           {monoid : Monoid B}
+  Fixpoint monoid_get_word {T}
+           {monoid : Monoid T}
            {monoid_opt : QueueMonoidOpt monoid bool}
            (sz : nat)
-           (b : B)
+           (b : T)
     : option (word sz) :=
     match sz with
     | 0 => Some WO
@@ -283,12 +281,12 @@ Section Word.
 
   Definition monoid_dequeue_word
          (sz : nat)
-         (b : B)
-  : option (word sz * B) := decode_word' sz b.
+         (b : T)
+  : option (word sz * T) := decode_word' sz b.
 
   Lemma monoid_dequeue_word_eq_decode_word' :
     forall (sz : nat)
-           (b : B),
+           (b : T),
       monoid_dequeue_word sz b = decode_word' sz b.
   Proof.
     reflexivity.
@@ -296,18 +294,18 @@ Section Word.
 
   Lemma monoid_dequeue_encode_word'
         (sz' : nat)
-    : forall (w : word sz') (ext : B),
+    : forall (w : word sz') (ext : T),
       monoid_dequeue_word sz' (mappend (encode_word' _ w mempty ) ext) = Some (w, ext).
   Proof.
     intros; unfold monoid_dequeue_word.
     apply decode_encode_word'.
   Qed.
 
-  Definition decode_unused_word' (s : nat) (b : B) : option (unit * B) :=
+  Definition decode_unused_word' (s : nat) (b : T) : option (unit * T) :=
     Ifopt monoid_dequeue_word s b as b' Then Some (tt, snd b') Else None.
 
   Definition decode_unused_word (sz' : nat)
-             (b : B) (cd : CacheDecode) : option (unit * B * CacheDecode) :=
+             (b : T) (cd : CacheDecode) : option (unit * T * CacheDecode) :=
     Ifopt decode_unused_word' sz' b as decoded Then Some (decoded, addD cd sz') Else None.
 
   Theorem unused_word_decode_correct sz'
@@ -346,11 +344,11 @@ End Word.
 
 Arguments format_unused_word {_ _ _ _ _} sz ctx _.
 
-Lemma monoid_get_encode_word' {B}
-      {monoid : Monoid B}
+Lemma monoid_get_encode_word' {T}
+      {monoid : Monoid T}
       {monoid_opt : QueueMonoidOpt monoid bool}
       (sz : nat)
-  : forall (w : word sz) (ext : B),
+  : forall (w : word sz) (ext : T),
     monoid_get_word sz (mappend (encode_word' _ w mempty) ext) = Some w.
 Proof.
   induction sz; simpl; intros; try shatter_word w; simpl in *.
@@ -372,7 +370,7 @@ Proof.
           (mappend (encode_word' sz (word_split_tl x0) mempty)
                      (mappend (enqueue_opt x mempty) ext))) as [ [? ?] | ];
             simpl in *; try discriminate.
-          destruct (monoid_get_word sz b0); try discriminate.
+          destruct (monoid_get_word sz t); try discriminate.
           injections.
           rewrite H0.
           simpl.
