src/Narcissus/BinLib/AlignedDecoders.v
@@ -91,6 +91,7 @@ Section AlignedDecoders.
 
   Variable addE_addE_plus :
     forall (ce : CacheFormat) (n m : nat), addE (addE ce n) m = addE ce (n + m).
+  Variable addE_0 : forall ce, addE ce 0 = ce.
 
   Lemma AlignedFormat2Char' {numBytes}
     : forall (w : word 16) ce ce' (c : _ -> Comp _) (v : Vector.t _ numBytes),
@@ -142,28 +143,11 @@ Section AlignedDecoders.
   Local Arguments split2 : simpl never.
 
   Lemma CorrectAlignedEncoderForFormat2Char
-    : forall (w : word 16),
-      CorrectAlignedEncoder
-        (format_word (monoidUnit := ByteString_QueueMonoidOpt) w)
-        (fun sz => AppendAlignedEncodeM (@SetCurrentByte _ _ sz (split2 8 8 w))
-                                        (SetCurrentByte (split1 8 8 w))).
+    : CorrectAlignedEncoder
+        (format_word (monoidUnit := ByteString_QueueMonoidOpt))
+        (fun n => @SetCurrentBytes _ _ n 16).
   Proof.
-    intro; pose proof (@format_words _ _ 8 8 addE_addE_plus w) as H';
-      eapply refine_CorrectAlignedEncoder.
-    unfold flip, pointwise_relation; intros.
-    instantiate (1 := (format_word (split2 8 8 (eq_rect (8 + 8) word w (8 + 8) (trans_plus_comm 8 8)))
-                                   ThenC (format_word (split1 8 8 (eq_rect (8 + 8) word w (8 + 8) (trans_plus_comm 8 8)))))).
-    rewrite (H' ce).
-    unfold compose, Bind2; simpl.
-    repeat setoid_rewrite Monad.refineEquiv_bind_bind;
-      repeat setoid_rewrite <- Monad.refine_bind_unit'.
-    f_equiv; intro.
-    eapply (CorrectAlignedEncoderForThenC
-              _ _ _
-              (fun sz => SetCurrentByte (n := sz) _)).
-    simpl in *|-*.
-    eapply (CorrectAlignedEncoderForFormatChar_f).
-    eapply (CorrectAlignedEncoderForFormatChar_f).
+    eapply CorrectAlignedEncoderForFormatNChar; eauto.
   Qed.
 
   Corollary AlignedDecode2Nat {C}
@@ -188,7 +172,7 @@ Section AlignedDecoders.
   Local Open Scope AlignedDecodeM_scope.
 
   Lemma AlignedDecodeNatM {C : Set}
-        (t : nat -> DecodeM C ByteString)
+        (t : nat -> DecodeM (C * _) ByteString)
         (t' : nat -> forall {numBytes}, AlignedDecodeM C numBytes)
     : (forall b, DecodeMEquivAlignedDecodeM (t b) (@t' b))
       -> DecodeMEquivAlignedDecodeM
@@ -253,12 +237,17 @@ Section AlignedDecoders.
   Qed.
 
   Lemma CorrectAlignedEncoderForFormatNat
-    : forall (n : nat),
-      CorrectAlignedEncoder
-        (format_nat 8 (monoidUnit := ByteString_QueueMonoidOpt) n)
-        (fun sz => @SetCurrentByte _ _ sz (natToWord 8 n)).
+    : CorrectAlignedEncoder
+        (format_nat 8 (monoidUnit := ByteString_QueueMonoidOpt))
+        (fun sz v idx n => @SetCurrentByte _ _ sz v idx (natToWord 8 n)).
   Proof.
-    eapply CorrectAlignedEncoderForFormatChar_f.
+    eapply refine_CorrectAlignedEncoder.
+    2: eapply CorrectAlignedEncoderForFormatChar_f.
+    unfold format_nat; intros.
+    intros ? ?.
+    unfold FMapFormat.Projection_Format, FMapFormat.FMap_Format in H.
+    rewrite unfold_computes in H.
+    destruct_ex; intuition; subst; eauto.
   Qed.
 
   Lemma optimize_under_if_opt {A ResultT}
@@ -1346,13 +1335,12 @@ Section AlignedDecoders.
           assert (n + S (m + sz) = n + S m + sz) by omega.
           (* Again, 8.4 compatibility problems. *)
           erewrite eq_rect_Vector_tl with (H' := H0).
-          erewrite eq_rect_Vector_tl with (H' := H1).
-          pose proof (IHn _ _ (Vector.tl v) H1 H0).
-          destruct ((Vector_split (n + m) sz (Vector.tl (eq_rect (n + S (m + sz)) (t A) (Vector.tl v) (S (n + m + sz)) H0)))) eqn: ?.
-          simpl in *; fold plus in *; rewrite Heqp, H2; simpl.
-          destruct (Vector_split (n + S m) sz (eq_rect (n + S (m + sz)) (Vector.t A) (Vector.tl v) (n + S m + sz) H1)) eqn: ?.
-          replace (plus_assoc n (S m) sz) with H1; simpl.
-          rewrite Heqp0; reflexivity.
+          erewrite eq_rect_Vector_tl with (H' := H).
+          pose proof (IHn _ _ (Vector.tl v) H0 H).
+          destruct ((Vector_split (n + m) sz (Vector.tl (eq_rect (n + S (m + sz)) (t A) (Vector.tl v) (S (n + m + sz)) H)))) eqn: ?.
+          simpl in *; fold plus in *; rewrite Heqp, H1; simpl.
+          destruct (Vector_split (n + S m) sz (eq_rect (n + S (m + sz)) (Vector.t A) (Vector.tl v) (n + S m + sz) H0)) eqn: ?.
+          replace (plus_assoc n (S m) sz) with H0; simpl; eauto.
           eapply Eqdep_dec.eq_proofs_unicity; intros; omega.
       + clear.
         revert H v.
@@ -1450,34 +1438,34 @@ Section AlignedDecoders.
       rewrite <- NPeano.leb_le in H1; congruence.
   Qed.
 
-
-  Definition calculate_Checksum {sz}
-    : AlignedEncodeM sz :=
-    fun v idx' ce =>
-      let checksum := InternetChecksum.Vector_checksum v in
-      (SetByteAt (split1 8 8 checksum) 10 >>
-                 SetByteAt (split2 8 8 checksum) 11)%AlignedEncodeM v idx' ce.
+  Definition calculate_Checksum {S} {sz}
+    : AlignedEncodeM (S := S) sz :=
+    (fun v =>
+      (let checksum := InternetChecksum.Vector_checksum v in
+      (fun v idx s => SetByteAt (n := sz) 10 v 0 (split1 8 8 checksum) ) >>
+      (fun v idx s => SetByteAt (n := sz) 11 v 0 (split2 8 8 checksum))) v)%AlignedEncodeM.
 
   Lemma CorrectAlignedEncoderForIPChecksumThenC
-        (format_A format_B : CacheFormat -> Comp (ByteString * CacheFormat))
+        {S}
+        (format_A format_B : FormatM S ByteString)
         (encode_A : forall sz, AlignedEncodeM sz)
         (encode_B : forall sz, AlignedEncodeM sz)
         (encoder_B_OK : CorrectAlignedEncoder format_B encode_B)
         (encoder_A_OK : CorrectAlignedEncoder format_A encode_A)
     : CorrectAlignedEncoder
-        (format_B ThenChecksum IPChecksum_Valid' OfSize 16 ThenCarryOn format_A)
+        (fun s => format_B s ThenChecksum IPChecksum_Valid' OfSize 16 ThenCarryOn (format_A s))
         (fun sz => encode_B sz >>
-                            SetCurrentByte (wzero 8) >>
-                            SetCurrentByte (wzero 8) >>
-                            encode_A sz >>
-                            calculate_Checksum)% AlignedEncodeM.
+                   (fun v idx s => SetCurrentByte v idx (wzero 8)) >>
+                   (fun v idx s => SetCurrentByte v idx (wzero 8)) >>
+                   encode_A sz >>
+                   calculate_Checksum)% AlignedEncodeM.
   Proof.
   Admitted.
 
   Lemma AlignedDecode_shift_if_bool {A B C : Type}
-        (decode_A : DecodeM A ByteString)
-        (decode_B : A -> DecodeM B ByteString)
-        (decode_C : A -> B -> DecodeM C ByteString)
+        (decode_A : DecodeM (A * _) ByteString)
+        (decode_B : A -> DecodeM (B * _) ByteString)
+        (decode_C : A -> B -> DecodeM (C * _) ByteString)
         (cond : A -> bool)
         (aligned_decoder : forall numBytes : nat, AlignedDecodeM C numBytes)
     : DecodeMEquivAlignedDecodeM
@@ -1502,9 +1490,9 @@ Section AlignedDecoders.
   Qed.
 
   Lemma AlignedDecode_shift_if_Sumb {A B C : Type}
-        (decode_A : DecodeM A ByteString)
-        (decode_B : A -> DecodeM B ByteString)
-        (decode_C : A -> B -> DecodeM C ByteString)
+        (decode_A : DecodeM (A * _) ByteString)
+        (decode_B : A -> DecodeM (B * _) ByteString)
+        (decode_C : A -> B -> DecodeM (C * _) ByteString)
         (P : A -> Prop)
         (cond : forall a, {P a} + {~P a})
         (aligned_decoder : forall numBytes : nat, AlignedDecodeM C numBytes)
@@ -1551,7 +1539,7 @@ Section AlignedDecoders.
   Lemma AlignedDecodeBind4CharM:
     forall (cache : Cache) (cacheAddNat : CacheAdd cache nat),
       (forall (cd : CacheDecode) (n m : nat), addD (addD cd n) m = addD cd (n + m)) ->
-      forall (C : Type) (t : word 32 -> DecodeM C ByteString)
+      forall (C : Type) (t : word 32 -> DecodeM (C * _) ByteString)
              (t' : word 32 -> forall numBytes : nat, AlignedDecodeM C numBytes),
         (forall b : word 32, DecodeMEquivAlignedDecodeM (t b) (t' b)) ->
         DecodeMEquivAlignedDecodeM
@@ -1571,8 +1559,8 @@ Section AlignedDecoders.
   Lemma AlignedDecode_CollapseWord' {A B}
     : forall (ResultT : Type) (sz sz' : nat)
              aligned_decoder
-             (decode_A : DecodeM A ByteString)
-             (decode_B : DecodeM B ByteString)
+             (decode_A : DecodeM (A * _) ByteString)
+             (decode_B : DecodeM (B * _) ByteString)
              (f : word sz -> A)
              (f' : word sz' -> B)
              (k : A -> B -> _ -> CacheDecode -> option (ResultT * _ * CacheDecode)),
@@ -1635,7 +1623,7 @@ Section AlignedDecoders.
 
   Lemma AlignedDecodeBindEnumM {A}
         {len}
-    : forall (t : Fin.t (S len) -> DecodeM A ByteString)
+    : forall (t : Fin.t (S len) -> DecodeM (A * _) ByteString)
              (t' : Fin.t (S len) -> forall numBytes : nat, AlignedDecodeM A numBytes)
              (tb : Vector.t (word 8) (S len)),
       (forall b2 : Fin.t (S len), DecodeMEquivAlignedDecodeM (t b2) (t' b2)) ->
@@ -1655,7 +1643,7 @@ Section AlignedDecoders.
   Admitted.
 
   Lemma AlignedDecodeBindUnused2CharM {C : Type}
-        (t : unit -> DecodeM C ByteString)
+        (t : unit -> DecodeM (C * _) ByteString)
         (t' : unit -> forall {numBytes}, AlignedDecodeM C numBytes)
     : (DecodeMEquivAlignedDecodeM (t ()) (@t' ()))
       -> DecodeMEquivAlignedDecodeM
@@ -1720,350 +1708,3 @@ Ltac encoder_reflexivity :=
     unify encoder' encoder''; unify store' store'';
     reflexivity
   end.
-(* 8 subgoals, subgoal 1 (ID 13672) *)
-
-(*   H : cache_inv_Property ?6326 *)
-(*         (fun P0 : () -> Prop => *)
-(*          (fun P : CacheDecode -> Prop => *)
-(*           (fun P1 : CacheDecode -> Prop => forall (b : nat) (cd : CacheDecode), P1 cd -> P1 (addD cd b)) P /\ *)
-(*           (fun P1 : CacheDecode -> Prop => *)
-(*            (fun P2 : CacheDecode -> Prop => forall (b : nat) (cd : CacheDecode), P2 cd -> P2 (addD cd b)) P1 /\ *)
-(*            (fun P2 : CacheDecode -> Prop => *)
-(*             (fun P3 : CacheDecode -> Prop => forall (b : nat) (cd : CacheDecode), P3 cd -> P3 (addD cd b)) P2 /\ *)
-(*             (fun P3 : CacheDecode -> Prop => *)
-(*              (fun P4 : CacheDecode -> Prop => forall (b : nat) (cd : CacheDecode), P4 cd -> P4 (addD cd b)) P3 /\ *)
-(*              (fun P4 : CacheDecode -> Prop => *)
-(*               (fun P5 : CacheDecode -> Prop => forall (b : nat) (cd : CacheDecode), P5 cd -> P5 (addD cd b)) P4 /\ *)
-(*               (fun P5 : CacheDecode -> Prop => *)
-(*                (fun P6 : CacheDecode -> Prop => forall (b : nat) (cd : CacheDecode), P6 cd -> P6 (addD cd b)) P5 /\ *)
-(*                (fun P6 : CacheDecode -> Prop => *)
-(*                 (fun P7 : CacheDecode -> Prop => forall (b : nat) (cd : CacheDecode), P7 cd -> P7 (addD cd b)) P6 /\ *)
-(*                 (fun P7 : CacheDecode -> Prop => *)
-(*                  (fun P8 : CacheDecode -> Prop => forall (b : nat) (cd : CacheDecode), P8 cd -> P8 (addD cd b)) *)
-(*                    P7 /\ (fun P8 : CacheDecode -> Prop => (fun .. => .., ..) P8 /\ (fun .. => .. /\ ..) P8) P7) *)
-(*                   P6) P5) P4) P3) P2) P1) P) P0 /\ *)
-(*          ?6529 P0 /\ *)
-(*          (forall (b : ByteString) (ctx u : ()) (b' : ByteString) (ctx' : ()), *)
-(*           decode_IPChecksum b ctx = Some (u, b', ctx') -> P0 ctx -> P0 ctx')) *)
-(*   StringId := "TotalLength" : string *)
-(*   StringId0 := "ID" : string *)
-(*   StringId1 := "DF" : string *)
-(*   StringId2 := "MF" : string *)
-(*   StringId3 := "FragmentOffset" : string *)
-(*   StringId4 := "TTL" : string *)
-(*   StringId5 := "Protocol" : string *)
-(*   StringId6 := "ICMP" : string *)
-(*   StringId7 := "TCP" : string *)
-(*   StringId8 := "UDP" : string *)
-(*   StringId9 := "SourceAddress" : string *)
-(*   StringId10 := "DestAddress" : string *)
-(*   StringId11 := "Options" : string *)
-(*   H0 : (fun _ : word 4 => True) (natToWord 4 4) *)
-(*   proj : nat *)
-(*   H1 : (fun n : nat => (n < pow2 4)%nat) proj *)
-(*   H2 : (fun _ : () => True) () *)
-(*   proj0 : word 16 *)
-(*   H3 : (fun _ : word 16 => True) proj0 *)
-(*   proj1 : word 16 *)
-(*   H4 : (fun _ : word 16 => True) proj1 *)
-(*   H5 : (fun _ : () => True) () *)
-(*   proj2 : bool *)
-(*   H6 : (fun _ : bool => True) proj2 *)
-(*   proj3 : bool *)
-(*   H7 : (fun _ : bool => True) proj3 *)
-(*   proj4 : word 13 *)
-(*   H8 : (fun _ : word 13 => True) proj4 *)
-(*   proj5 : word 8 *)
-(*   H9 : (fun _ : word 8 => True) proj5 *)
-(*   proj6 : Fin.t 3 *)
-(*   H10 : (fun _ : Fin.t 3 => True) proj6 *)
-(*   H11 : cache_inv_Property ?6326 ?11546 *)
-(*   ============================ *)
-(*    forall *)
-(*      a' : nat * *)
-(*           (id (word 16) * *)
-(*            (id (word 16) * *)
-(*             (id bool * *)
-(*              (id bool * (id (word 13) * (id (word 8) * (id (EnumType ("ICMP" :: "TCP" :: ["UDP"])) * ?6966))))))), *)
-(*    ((((((((?9072 a' /\ (fst a' < pow2 4)%nat) /\ fst a' = proj) /\ fst (snd a') = proj0) /\ *)
-(*         fst (snd (snd a')) = proj1) /\ fst (snd (snd (snd a'))) = proj2) /\ *)
-(*       fst (snd (snd (snd (snd a')))) = proj3) /\ fst (snd (snd (snd (snd (snd a'))))) = proj4) /\ *)
-(*     fst (snd (snd (snd (snd (snd (snd a')))))) = proj5) /\ *)
-(*    fst (snd (snd (snd (snd (snd (snd (snd a'))))))) = proj6 ->  *)
-(*    a' = ?13671 *)
-
-(* subgoal 2 (ID 13673) is: *)
-(*  decides ?13670 *)
-(*    (((((((((?9072 ?13671 /\ (fst ?13671 < pow2 4)%nat) /\ fst ?13671 = proj) /\ fst (snd ?13671) = proj0) /\ *)
-(*          fst (snd (snd ?13671)) = proj1) /\ fst (snd (snd (snd ?13671))) = proj2) /\ *)
-(*        fst (snd (snd (snd (snd ?13671)))) = proj3) /\  *)
-(*       fst (snd (snd (snd (snd (snd ?13671))))) = proj4) /\  *)
-(*      fst (snd (snd (snd (snd (snd (snd ?13671)))))) = proj5) /\ *)
-(*     fst (snd (snd (snd (snd (snd (snd (snd ?13671))))))) = proj6) *)
-(* subgoal 3 (ID 6524) is: *)
-(*  forall data : IPv4_Packet, *)
-(*  ((|data!StringId11 |) < 11)%nat /\ *)
-(*  (S (S (S (S (S (S (S (S (S (S (S (S (S (S (S (S (S (S (S (S (4 * (..))))))))))))))))))))) < *)
-(*   wordToNat data!StringId)%nat -> *)
-(*  (fun *)
-(*     a : nat * *)
-(*         (id (word 16) * *)
-(*          (id (word 16) * *)
-(*           (id bool * *)
-(*            (id bool * (id (word 13) * (id (word 8) * (id (EnumType ("ICMP" :: "TCP" :: ["UDP"])) * ?6966))))))) => *)
-(*   (fun *)
-(*      data0 : nat * *)
-(*              (id (word 16) * *)
-(*               (id (word 16) * *)
-(*                (id bool * *)
-(*                 (id bool * (id (word 13) * (id (word 8) * (id (EnumType ("ICMP" :: "TCP" :: ["UDP"])) * ?6966))))))) => *)
-(*    ?9072 data0 /\ *)
-(*    (fun *)
-(*       p : nat * *)
-(*           (id (word 16) * *)
-(*            (id (word 16) * *)
-(*             (id bool * *)
-(*              (id bool * (id (word 13) * (id (word 8) * (id (EnumType ("ICMP" :: "TCP" :: ["UDP"])) * ?6966))))))) => *)
-(*     (fun n : nat => (n < pow2 4)%nat) (fst p)) data0) a) *)
-(*    ((fun H0 : IPv4_Packet => *)
-(*      (IPv4_Packet_Header_Len H0, *)
-(*      (fun H1 : IPv4_Packet => *)
-(*       (prim_fst H1, *)
-(*       (fun H2 : IPv4_Packet => *)
-(*        ((fun a : IPv4_Packet => prim_fst (prim_snd a)) H2, *)
-(*        (fun H3 : IPv4_Packet => *)
-(*         ((fun a : IPv4_Packet => prim_fst (prim_snd (prim_snd a))) H3, *)
-(*         (fun H4 : IPv4_Packet => *)
-(*          ((fun a : IPv4_Packet => prim_fst (prim_snd (prim_snd (prim_snd a)))) H4, *)
-(*          (fun H5 : IPv4_Packet => *)
-(*           ((fun a : IPv4_Packet => prim_fst (prim_snd (prim_snd (prim_snd (prim_snd a))))) H5, *)
-(*           (fun H6 : IPv4_Packet => *)
-(*            ((fun a : IPv4_Packet => prim_fst (prim_snd (prim_snd (prim_snd (prim_snd (prim_snd a)))))) H6, *)
-(*            (fun H7 : IPv4_Packet => *)
-(*             ((fun a : IPv4_Packet => prim_fst (prim_snd (prim_snd (prim_snd (..))))) H7, ?6964 H7)) H6)) H5)) H4)) *)
-(*           H3)) H2)) H1)) H0)) data) *)
-(* subgoal 4 (ID 6525) is: *)
-(*  forall *)
-(*    (a' : nat * *)
-(*          (id (word 16) * *)
-(*           (id (word 16) * *)
-(*            (id bool * *)
-(*             (id bool * (id (word 13) * (id (word 8) * (id (EnumType ("ICMP" :: "TCP" :: ["UDP"])) * ?6966)))))))) *)
-(*    (b : ByteString) (a : IPv4_Packet) (ce ce' ce'' : CacheFormat)  *)
-(*    (b' b'' : ByteString) (c : word 16), *)
-(*  (fun *)
-(*     (a'0 : nat * *)
-(*            (id (word 16) * *)
-(*             (id (word 16) * *)
-(*              (id bool * *)
-(*               (id bool * (id (word 13) * (id (word 8) * (id (EnumType ("ICMP" :: "TCP" :: ["UDP"])) * ?6966)))))))) *)
-(*     (env : CacheFormat) => *)
-(*   (format_word (natToWord 4 4) *)
-(*    ThenC (fun *)
-(*             (aa' : nat * *)
-(*                    (id (word 16) * *)
-(*                     (id (word 16) * *)
-(*                      (id bool * *)
-(*                       (id bool * *)
-(*                        (id (word 13) * *)
-(*                         (id (word 8) * (id (EnumType (StringId6 :: StringId7 :: [StringId8])) * ?6966)))))))) *)
-(*             (env0 : CacheFormat) => *)
-(*           (format_nat 4 (fst aa') *)
-(*            ThenC (fun *)
-(*                     (a'1 : id (word 16) * *)
-(*                            (id (word 16) * *)
-(*                             (id bool * *)
-(*                              (id bool * *)
-(*                               (id (word 13) * *)
-(*                                (id (word 8) * (id (EnumType (StringId6 :: StringId7 :: [StringId8])) * ?6966))))))) *)
-(*                     (env1 : CacheFormat) => *)
-(*                   (format_unused_word 8 *)
-(*                    ThenC (fun *)
-(*                             (aa'0 : id (word 16) * *)
-(*                                     (id (word 16) * *)
-(*                                      (id bool * *)
-(*                                       (id bool * *)
-(*                                        (id (word 13) * *)
-(*                                         (id (word 8) * *)
-(*                                          (id (EnumType (StringId6 :: StringId7 :: [StringId8])) * ?6966))))))) *)
-(*                             (env2 : CacheFormat) => *)
-(*                           (format_word (fst aa'0) *)
-(*                            ThenC (fun *)
-(*                                     (aa'1 : id (word 16) * *)
-(*                                             (id bool * *)
-(*                                              (id bool * *)
-(*                                               (id (word 13) * (id (word 8) * (id (EnumType (..)) * ?6966)))))) *)
-(*                                     (env3 : CacheFormat) => *)
-(*                                   (format_word (fst aa'1) *)
-(*                                    ThenC (fun *)
-(*                                             (a'2 : id bool * (id bool * (id (word 13) * (id (..) * (.. * ..))))) *)
-(*                                             (env4 : CacheFormat) => *)
-(*                                           (format_unused_word 1 *)
-(*                                            ThenC (fun (aa'2 : id bool * (.. * ..)) (env5 : CacheFormat) => *)
-(*                                                   (format_bool (..) ThenC (..) (..)) env5) a'2) env4)  *)
-(*                                            (snd aa'1)) env3)  *)
-(*                                    (snd aa'0)) env2) a'1) env1)  *)
-(*                    (snd aa')) env0) a'0) env) a' ce ↝  *)
-(*  (b', ce') -> *)
-(*  (fun H0 : IPv4_Packet => *)
-(*   (IPv4_Packet_Header_Len H0, *)
-(*   (fun H1 : IPv4_Packet => *)
-(*    (prim_fst H1, *)
-(*    (fun H2 : IPv4_Packet => *)
-(*     ((fun a0 : IPv4_Packet => prim_fst (prim_snd a0)) H2, *)
-(*     (fun H3 : IPv4_Packet => *)
-(*      ((fun a0 : IPv4_Packet => prim_fst (prim_snd (prim_snd a0))) H3, *)
-(*      (fun H4 : IPv4_Packet => *)
-(*       ((fun a0 : IPv4_Packet => prim_fst (prim_snd (prim_snd (prim_snd a0)))) H4, *)
-(*       (fun H5 : IPv4_Packet => *)
-(*        ((fun a0 : IPv4_Packet => prim_fst (prim_snd (prim_snd (prim_snd (prim_snd a0))))) H5, *)
-(*        (fun H6 : IPv4_Packet => *)
-(*         ((fun a0 : IPv4_Packet => prim_fst (prim_snd (prim_snd (prim_snd (prim_snd (prim_snd a0)))))) H6, *)
-(*         (fun H7 : IPv4_Packet => *)
-(*          ((fun a0 : IPv4_Packet => prim_fst (prim_snd (prim_snd (prim_snd (..))))) H7, ?6964 H7)) H6)) H5)) H4)) *)
-(*        H3)) H2)) H1)) H0)) a = a' -> *)
-(*  ((|a!StringId11 |) < 11)%nat /\ *)
-(*  (S (S (S (S (S (S (S (S (S (S (S (S (S (S (S (S (S (S (S (S (..)))))))))))))))))))) < wordToNat a!StringId)%nat -> *)
-(*  (format_word a!StringId9 *)
-(*   ThenC format_word a!StringId10 *)
-(*         ThenC format_list format_word a!StringId11 ThenC (fun e : () => ret (ByteString_id, e))) ce' *)
-(*  ↝ (b'', ce'') -> *)
-(*  True -> *)
-(*  {c0 : word 16 | *)
-(*  forall ext : ByteString, *)
-(*  IPChecksum_Valid' *)
-(*    (bin_measure *)
-(*       (mappend b' *)
-(*          (mappend *)
-(*             (format_checksum ByteString AlignedByteString.ByteStringQueueMonoid ByteString_QueueMonoidOpt 16 c0) *)
-(*             b''))) *)
-(*    (mappend *)
-(*       (mappend b' *)
-(*          (mappend *)
-(*             (format_checksum ByteString AlignedByteString.ByteStringQueueMonoid ByteString_QueueMonoidOpt 16 c0) *)
-(*             b'')) ext)} ↝ c -> *)
-(*  ?6512 a' *)
-(*    (mappend *)
-(*       (mappend *)
-(*          (format_checksum ByteString AlignedByteString.ByteStringQueueMonoid ByteString_QueueMonoidOpt 16 c) b'') *)
-(*       b) *)
-(* subgoal 5 (ID 6526) is: *)
-(*  forall *)
-(*    proj : nat * *)
-(*           (id (word 16) * *)
-(*            (id (word 16) * *)
-(*             (id bool * *)
-(*              (id bool * (id (word 13) * (id (word 8) * (id (EnumType ("ICMP" :: "TCP" :: ["UDP"])) * ?6966))))))), *)
-(*  (fun *)
-(*     a : nat * *)
-(*         (id (word 16) * *)
-(*          (id (word 16) * *)
-(*           (id bool * *)
-(*            (id bool * (id (word 13) * (id (word 8) * (id (EnumType ("ICMP" :: "TCP" :: ["UDP"])) * ?6966))))))) => *)
-(*   (fun *)
-(*      data : nat * *)
-(*             (id (word 16) * *)
-(*              (id (word 16) * *)
-(*               (id bool * *)
-(*                (id bool * (id (word 13) * (id (word 8) * (id (EnumType ("ICMP" :: "TCP" :: ["UDP"])) * ?6966))))))) => *)
-(*    ?9072 data /\ *)
-(*    (fun *)
-(*       p : nat * *)
-(*           (id (word 16) * *)
-(*            (id (word 16) * *)
-(*             (id bool * *)
-(*              (id bool * (id (word 13) * (id (word 8) * (id (EnumType ("ICMP" :: "TCP" :: ["UDP"])) * ?6966))))))) => *)
-(*     (fun n : nat => (n < pow2 4)%nat) (fst p)) data) a) proj -> *)
-(*  cache_inv_Property ?6326 ?6529 -> *)
-(*  CorrectDecoder AlignedByteString.ByteStringQueueMonoid *)
-(*    (fun data : IPv4_Packet => *)
-(*     (((|data!StringId11 |) < 11)%nat /\ *)
-(*      (S (S (S (S (S (S (S (S (S (S (S (S (S (S (S (S (S (S (..)))))))))))))))))) < wordToNat data!StringId)%nat) /\ *)
-(*     (fun H0 : IPv4_Packet => *)
-(*      (IPv4_Packet_Header_Len H0, *)
-(*      (fun H1 : IPv4_Packet => *)
-(*       (prim_fst H1, *)
-(*       (fun H2 : IPv4_Packet => *)
-(*        ((fun a : IPv4_Packet => prim_fst (prim_snd a)) H2, *)
-(*        (fun H3 : IPv4_Packet => *)
-(*         ((fun a : IPv4_Packet => prim_fst (prim_snd (prim_snd a))) H3, *)
-(*         (fun H4 : IPv4_Packet => *)
-(*          ((fun a : IPv4_Packet => prim_fst (prim_snd (prim_snd (prim_snd a)))) H4, *)
-(*          (fun H5 : IPv4_Packet => *)
-(*           ((fun a : IPv4_Packet => prim_fst (prim_snd (prim_snd (prim_snd (prim_snd a))))) H5, *)
-(*           (fun H6 : IPv4_Packet => *)
-(*            ((fun a : IPv4_Packet => prim_fst (prim_snd (prim_snd (prim_snd (..))))) H6, *)
-(*            (fun H7 : IPv4_Packet => ((fun a : IPv4_Packet => prim_fst (prim_snd (..))) H7, ?6964 H7)) H6)) H5)) *)
-(*            H4)) H3)) H2)) H1)) H0)) data = proj) (fun (_ : IPv4_Packet) (_ : ByteString) => True) *)
-(*    (fun data : IPv4_Packet => *)
-(*     format_word data!StringId9 *)
-(*     ThenC format_word data!StringId10 *)
-(*           ThenC format_list format_word data!StringId11 ThenC (fun e : () => ret (ByteString_id, e))) *)
-(*    (?6507 proj) ?6326 *)
-(* subgoal 6 (ID 6333) is: *)
-(*  cache_inv_Property ?6326 *)
-(*    (fun P0 : () -> Prop => *)
-(*     (fun P : CacheDecode -> Prop => *)
-(*      (fun P1 : CacheDecode -> Prop => forall (b : nat) (cd : CacheDecode), P1 cd -> P1 (addD cd b)) P /\ *)
-(*      (fun P1 : CacheDecode -> Prop => *)
-(*       (fun P2 : CacheDecode -> Prop => forall (b : nat) (cd : CacheDecode), P2 cd -> P2 (addD cd b)) P1 /\ *)
-(*       (fun P2 : CacheDecode -> Prop => *)
-(*        (fun P3 : CacheDecode -> Prop => forall (b : nat) (cd : CacheDecode), P3 cd -> P3 (addD cd b)) P2 /\ *)
-(*        (fun P3 : CacheDecode -> Prop => *)
-(*         (fun P4 : CacheDecode -> Prop => forall (b : nat) (cd : CacheDecode), P4 cd -> P4 (addD cd b)) P3 /\ *)
-(*         (fun P4 : CacheDecode -> Prop => *)
-(*          (fun P5 : CacheDecode -> Prop => forall (b : nat) (cd : CacheDecode), P5 cd -> P5 (addD cd b)) P4 /\ *)
-(*          (fun P5 : CacheDecode -> Prop => *)
-(*           (fun P6 : CacheDecode -> Prop => forall (b : nat) (cd : CacheDecode), P6 cd -> P6 (addD cd b)) P5 /\ *)
-(*           (fun P6 : CacheDecode -> Prop => *)
-(*            (fun P7 : CacheDecode -> Prop => forall (b : nat) (cd : CacheDecode), P7 cd -> P7 (addD cd b)) P6 /\ *)
-(*            (fun P7 : CacheDecode -> Prop => *)
-(*             (fun P8 : CacheDecode -> Prop => forall (b : nat) (cd : CacheDecode), P8 cd -> P8 (addD cd b)) P7 /\ *)
-(*             (fun P8 : CacheDecode -> Prop => *)
-(*              (fun P9 : CacheDecode -> Prop => forall (b : nat) (cd : CacheDecode), P9 cd -> P9 (..)) P8 /\ *)
-(*              (fun P9 : CacheDecode -> Prop => (.. => ..) P9 /\ (.. => ..) P9) P8) P7) P6) P5) P4) P3) P2) P1) P) *)
-(*       P0 /\ *)
-(*     ?6529 P0 /\ *)
-(*     (forall (b : ByteString) (ctx u : ()) (b' : ByteString) (ctx' : ()), *)
-(*      decode_IPChecksum b ctx = Some (u, b', ctx') -> P0 ctx -> P0 ctx')) *)
-(* subgoal 7 (ID 6338) is: *)
-(*  (fun (bin : ByteString) (env : CacheDecode) => *)
-(*   if IPChecksum_Valid_dec (IPv4_Packet_formatd_measure bin) bin *)
-(*   then *)
-(*    `(proj, rest, env') <- (fun (bin0 : ByteString) (env0 : CacheDecode) => *)
-(*                            `(a, rest, env') <- decode_word bin0 env0; *)
-(*                            (if DecideableEnsembles.A_eq_dec a (natToWord 4 4) *)
-(*                             then *)
-(*                              (fun (bin1 : ByteString) (env1 : CacheDecode) => *)
-(*                               `(proj, rest0, env'0) <-  *)
-(*                               decode_nat 4 bin1 env1; *)
-(*                               (fun (proj0 : nat) (bin2 : ByteString) (env2 : CacheDecode) => *)
-(*                                `(a0, rest1, env'1) <-  *)
-(*                                decode_unused_word 8 bin2 env2; *)
-(*                                (if DecideableEnsembles.A_eq_dec a0 () *)
-(*                                 then *)
-(*                                  (fun (bin3 : ByteString) (env3 : CacheDecode) => *)
-(*                                   `(proj1, rest2, env'2) <-  *)
-(*                                   decode_word bin3 env3; *)
-(*                                   (fun (proj2 : word 16) (bin4 : ByteString) (env4 : CacheDecode) => *)
-(*                                    `(proj3, rest3, env'3) <-  *)
-(*                                    decode_word bin4 env4; *)
-(*                                    (fun (proj4 : word 16) (bin5 : ByteString) (env5 : CacheDecode) => *)
-(*                                     `(a1, rest4, env'4) <-  *)
-(*                                     decode_unused_word 1 bin5 env5; *)
-(*                                     (if DecideableEnsembles.A_eq_dec a1 () *)
-(*                                      then *)
-(*                                       (fun (bin6 : ByteString) (env6 : CacheDecode) => *)
-(*                                        `(proj5, rest5, env'5) <-  *)
-(*                                        decode_bool bin6 env6; *)
-(*                                        (.. => ..) proj5 rest5 env'5) rest4 env'4 *)
-(*                                      else None)) proj3 rest3 env'3) proj1 rest2 env'2) rest1 env'1 *)
-(*                                 else None)) proj rest0 env'0) rest env' *)
-(*                             else None)) bin env; *)
-(*    `(_, rest', env'0) <- decode_IPChecksum rest env'; *)
-(*    ?6507 proj rest' env'0 *)
-(*   else None) b cd = ?6324 b cd *)
-(* subgoal 8 (ID 6335) is: *)
-(*  DecodeMEquivAlignedDecodeM ?6324 ?6325 *)
-
-(* (dependent evars: ?6321 using , ?6322 using , ?6323 using ?6506 ?6493 ?6492 ?6491 , ?6324 open, ?6325 open, ?6326 open, ?6327 using ?6529 ?6528 , ?6339 using , ?6486 using ?6492 , ?6491 using , ?6492 using ?6498 , ?6493 using ?8533 ?8532 ?8531 ?8530 ?8529 ?8528 , ?6498 using ?6572 ?6571 , ?6505 using , ?6506 using ?6507 , ?6507 open, ?6508 using ?6528 , ?6509 using ?6529 , ?6510 using ?6570 ?6569 ?6568 ?6567 ?6566 , ?6511 using ?8535 ?6966 , ?6512 open, ?6513 using ?6542 ?6498 , ?6514 using ?7035 ?7034 , ?6515 using ?8103 ?8102 , ?6528 using ?8525 ?8524 , ?6529 open, ?6536 using ?6542 , ?6542 using ?6594 ?6572 , ?6561 using ?6566 , ?6562 using ?6567 , ?6566 using ?6571 , ?6567 using ?6572 , ?6568 using , ?6569 using , ?6570 using ?6637 ?6636 ?6635 ?6634 ?6633 , ?6571 using , ?6572 using ?6639 ?6638 , ?6573 using , ?6574 using ?6594 , ?6594 using ?6609 ?6572 , ?6603 using ?6609 , ?6609 using ?6661 ?6639 , ?6628 using ?6633 , ?6629 using ?6634 , ?6633 using ?6638 , ?6634 using ?6639 , ?6635 using , ?6636 using , ?6637 using ?6689 ?6688 ?6687 ?6686 ?6685 , ?6638 using , ?6639 using ?6691 ?6690 , ?6640 using , ?6641 using ?6661 , ?6661 using ?6713 ?6691 , ?6680 using ?6685 , ?6681 using ?6686 , ?6685 using ?6690 , ?6686 using ?6691 , ?6687 using , ?6688 using , ?6689 using ?6756 ?6755 ?6754 ?6753 ?6752 , ?6690 using , ?6691 using ?6758 ?6757 , ?6692 using , ?6693 using ?6713 , ?6713 using ?6728 ?6691 , ?6722 using ?6728 , ?6728 using ?6780 ?6758 , ?6747 using ?6752 , ?6748 using ?6753 , ?6752 using ?6757 , ?6753 using ?6758 , ?6754 using , ?6755 using , ?6756 using ?6808 ?6807 ?6806 ?6805 ?6804 , ?6757 using , ?6758 using ?6810 ?6809 , ?6759 using , ?6760 using ?6780 , ?6780 using ?6832 ?6810 , ?6799 using ?6804 , ?6800 using ?6805 , ?6804 using ?6809 , ?6805 using ?6810 , ?6806 using , ?6807 using , ?6808 using ?6860 ?6859 ?6858 ?6857 ?6856 , ?6809 using , ?6810 using ?6862 ?6861 , ?6811 using , ?6812 using ?6832 , ?6832 using ?6884 ?6862 , ?6851 using ?6856 , ?6852 using ?6857 , ?6856 using ?6861 , ?6857 using ?6862 , ?6858 using , ?6859 using , ?6860 using ?6912 ?6911 ?6910 ?6909 ?6908 , ?6861 using , ?6862 using ?6914 ?6913 , ?6863 using , ?6864 using ?6884 , ?6884 using ?6936 ?6914 , ?6903 using ?6908 , ?6904 using ?6909 , ?6908 using ?6913 , ?6909 using ?6914 , ?6910 using , ?6911 using , ?6912 using ?6964 ?6963 ?6962 ?6961 ?6960 , ?6913 using , ?6914 using ?6966 ?6965 , ?6915 using , ?6916 using ?6936 , ?6936 using ?6988 ?6966 , ?6955 using ?6960 , ?6956 using ?6961 , ?6960 using ?6965 , ?6961 using ?6966 , ?6962 using , ?6963 using , ?6964 open, ?6965 using , ?6966 open, ?6967 using , ?6968 using ?6988 , ?6988 using ?6966 , ?7034 using , ?7035 using ?7128 ?7127 , ?7127 using , ?7128 using ?7221 ?7220 , ?7220 using , ?7221 using ?7305 ?7304 , ?7304 using , ?7305 using ?7398 ?7397 , ?7397 using , ?7398 using ?7491 ?7490 , ?7490 using , ?7491 using ?7575 ?7574 , ?7574 using , ?7575 using ?7663 ?7662 , ?7662 using , ?7663 using ?7751 ?7750 , ?7750 using , ?7751 using ?7844 ?7843 , ?7843 using , ?7844 using ?7937 ?7936 , ?7936 using , ?7937 using , ?8102 using , ?8103 using ?8196 ?8195 , ?8195 using , ?8196 using ?8289 ?8288 , ?8288 using ?8365 , ?8289 using , ?8354 using ?8364 ?8363 ?8362 , ?8355 using ?8362 , ?8362 using , ?8363 using , ?8364 using ?8365 , ?8365 using , ?8516 using ?8530 , ?8517 using ?8529 , ?8518 using ?8528 , ?8520 using , ?8524 using , ?8525 using ?8834 ?8833 , ?8528 using , ?8529 using , ?8530 using ?6966 , ?8531 using ?8689 ?8688 ?8687 ?8686 ?8685 ?8684 , ?8532 using , ?8533 using ?8841 ?8840 ?8839 ?8838 ?8837 , ?8535 using ?9072 ?6966 , ?8536 using ?8542 , ?8537 using ?8543 , ?8542 using , ?8543 using , ?8678 using ?8685 , ?8679 using ?8686 , ?8681 using ?8688 , ?8684 using , ?8685 using , ?8686 using , ?8687 using , ?8688 using , ?8689 using , ?8826 using ?8839 , ?8827 using ?8838 , ?8828 using ?8837 , ?8829 using , ?8833 using , ?8834 using ?9159 ?9158 , ?8837 using , ?8838 using , ?8839 using ?6966 , ?8840 using , ?8841 using ?9169 ?9168 ?9167 ?9166 ?9165 ?9164 ?9163 , ?8842 using ?8848 , ?8843 using ?8849 , ?8848 using , ?8849 using , ?9067 using ?9072 , ?9072 open, ?9150 using ?9165 , ?9151 using ?9164 , ?9152 using ?9163 , ?9154 using , ?9158 using , ?9159 using ?9442 ?9441 , ?9163 using , ?9164 using , ?9165 using ?6966 , ?9166 using , ?9167 using , ?9168 using , ?9169 using ?9449 ?9448 ?9447 ?9446 ?9445 , ?9170 using ?9176 , ?9171 using ?9177 , ?9176 using , ?9177 using , ?9434 using ?9447 , ?9435 using ?9446 , ?9436 using ?9445 , ?9437 using , ?9441 using , ?9442 using ?9755 ?9754 , ?9445 using , ?9446 using , ?9447 using ?6966 , ?9448 using ?9603 ?9602 ?9601 ?9600 ?9599 ?9598 , ?9449 using ?9762 ?9761 ?9760 ?9759 ?9758 , ?9450 using ?9456 , ?9451 using ?9457 , ?9456 using , ?9457 using , ?9592 using ?9599 , ?9593 using ?9600 , ?9595 using ?9602 , ?9598 using , ?9599 using , ?9600 using , ?9601 using , ?9602 using , ?9603 using , ?9747 using ?9760 , ?9748 using ?9759 , ?9749 using ?9758 , ?9750 using , ?9754 using , ?9755 using ?10051 ?10050 , ?9758 using , ?9759 using , ?9760 using ?6966 , ?9761 using ?9916 ?9915 ?9914 ?9913 ?9912 ?9911 , ?9762 using ?10061 ?10060 ?10059 ?10058 ?10057 ?10056 ?10055 , ?9763 using ?9769 , ?9764 using ?9770 , ?9769 using , ?9770 using , ?9905 using ?9912 , ?9906 using ?9913 , ?9908 using ?9915 , ?9911 using , ?9912 using , ?9913 using , ?9914 using , ?9915 using , ?9916 using , ?10042 using ?10057 , ?10043 using ?10056 , ?10044 using ?10055 , ?10046 using , ?10050 using , ?10051 using ?10334 ?10333 , ?10055 using , ?10056 using , ?10057 using ?6966 , ?10058 using , ?10059 using , ?10060 using , ?10061 using ?10341 ?10340 ?10339 ?10338 ?10337 , ?10062 using ?10068 , ?10063 using ?10069 , ?10068 using , ?10069 using , ?10326 using ?10339 , ?10327 using ?10338 , ?10328 using ?10337 , ?10329 using , ?10333 using , ?10334 using ?10627 ?10626 , ?10337 using , ?10338 using , ?10339 using ?6966 , ?10340 using ?10475 ?10474 ?10473 ?10472 ?10471 , ?10341 using ?10634 ?10633 ?10632 ?10631 ?10630 , ?10342 using ?10348 , ?10343 using ?10349 , ?10348 using , ?10349 using , ?10465 using ?10471 , ?10466 using ?10472 , ?10468 using ?10474 , ?10471 using , ?10472 using , ?10473 using , ?10474 using , ?10475 using , ?10619 using ?10632 , ?10620 using ?10631 , ?10621 using ?10630 , ?10622 using , ?10626 using , ?10627 using ?10920 ?10919 , ?10630 using , ?10631 using , ?10632 using ?6966 , ?10633 using ?10768 ?10767 ?10766 ?10765 ?10764 , ?10634 using ?10927 ?10926 ?10925 ?10924 ?10923 , ?10635 using ?10641 , ?10636 using ?10642 , ?10641 using , ?10642 using , ?10758 using ?10764 , ?10759 using ?10765 , ?10761 using ?10767 , ?10764 using , ?10765 using , ?10766 using , ?10767 using , ?10768 using , ?10912 using ?10925 , ?10913 using ?10924 , ?10914 using ?10923 , ?10915 using , ?10919 using , ?10920 using ?11233 ?11232 , ?10923 using , ?10924 using , ?10925 using ?6966 , ?10926 using ?11081 ?11080 ?11079 ?11078 ?11077 ?11076 , ?10927 using ?11240 ?11239 ?11238 ?11237 ?11236 , ?10928 using ?10934 , ?10929 using ?10935 , ?10934 using , ?10935 using , ?11070 using ?11077 , ?11071 using ?11078 , ?11073 using ?11080 , ?11076 using , ?11077 using , ?11078 using , ?11079 using , ?11080 using , ?11081 using , ?11225 using ?11238 , ?11226 using ?11237 , ?11227 using ?11236 , ?11228 using , ?11232 using , ?11233 using ?11546 ?11545 , ?11236 using , ?11237 using , ?11238 using ?6966 , ?11239 using ?11394 ?11393 ?11392 ?11391 ?11390 ?11389 , ?11240 using ?11553 ?11552 ?11551 ?11550 ?11549 , ?11241 using ?11247 , ?11242 using ?11248 , ?11247 using , ?11248 using , ?11383 using ?11390 , ?11384 using ?11391 , ?11386 using ?11393 , ?11389 using , ?11390 using , ?11391 using , ?11392 using , ?11393 using , ?11394 using , ?11538 using ?11551 , ?11539 using ?11550 , ?11540 using ?11549 , ?11541 using , ?11545 using , ?11546 open, ?11549 using , ?11550 using , ?11551 using ?6966 , ?11552 using ?11688 ?11687 ?11686 ?11685 ?11684 , ?11553 using ?13671 ?13670 ?13669 ?13668 ?13667 , ?11554 using ?11560 , ?11555 using ?11561 , ?11560 using , ?11561 using , ?11678 using ?11684 , ?11679 using ?11685 , ?11681 using ?11687 , ?11684 using , ?11685 using , ?11686 using , ?11687 using , ?11688 using , ?13662 using ?13668 , ?13667 using , ?13668 using ?6966 , ?13669 using , ?13670 open, ?13671 open,) *)
